Risc0/Map.lean
@@ -1,0 +1,126 @@
+import Mathlib.Data.Option.Basic
+
+namespace Risc0
+
+def Map (α : Type) (β : Type) := α → Option β
+
+namespace Map
+
+section Map
+
+variable {α : Type} [DecidableEq α] {β : Type}
+
+def empty : Map α β := λ _ => none
+
+def update (m : Map α β) (k : α) (v : β) : Map α β :=
+  λ x => if x = k then v else m x
+
+end Map
+
+end Map
+
+notation:61 m "[" k:61 "]" " := " v:49 => Map.update m k v
+
+section Map.Instances
+
+variable {α β : Type} [DecidableEq α]
+
+-- k ∈ m
+instance : Membership α (Map α β) := ⟨λ k m => (m k).isSome⟩
+
+-- m[k]
+instance : GetElem (Map α β) α (Option β) (λ _ _ => True) := ⟨λ m k _ => m k⟩
+
+end Map.Instances
+
+namespace Map
+
+section Map
+
+variable {α : Type} [DecidableEq α] {β : Type}
+         {m : Map α β} {k k' : α} {v v' : β}
+
+def get (h : k ∈ m) := m[k].get h
+
+def get! [Inhabited β] (k : α) := m[k].get!
+
+lemma get_def (h : k ∈ m) : m.get h = m[k].get h := rfl
+
+def fromList (l : List (α × β)) : Map α β :=
+  match l with
+    | [] => Map.empty
+    | (k, v) :: xs => Map.update (Map.fromList xs) k v
+
+@[simp]
+lemma getElem_def : m[k] = m k := rfl
+
+@[simp]
+lemma fromList_nil : fromList ([] : List (α × β)) = Map.empty := rfl
+
+@[simp]
+lemma fromList_cons {l : List (α × β)} :
+  fromList ((k, v) :: l) = Map.update (Map.fromList l) k v := rfl
+
+@[simp]
+lemma update_get : (m[k] := v)[k] = v := by simp [update]
+
+@[simp]
+lemma empty_get : (@Map.empty α β)[k] = none := by rfl
+
+lemma update_get_skip (h : k ≠ k') (h₁ : m[k] = some v) :
+  (m[k'] := v')[k] = some v := by simp [update, h, getElem_def ▸ h₁]
+
+-- Membership lemmas.
+lemma mem_def : (x ∈ m) = m[x].isSome := rfl
+
+@[simp]
+lemma mem_update_self : k ∈ m[k] := v := by
+  rw [mem_def, Option.isSome_iff_exists, update_get]; use v
+
+lemma mem_skip (h : k ∈ m) : k ∈ m[k'] := v := by simp [mem_def, update]; aesop
+
+@[simp]
+lemma not_mem_empty : k ∉ @empty α β :=
+  λ contra => by simp [Map.mem_def, empty] at contra
+
+@[simp]
+lemma not_empty_eq_some : ¬Option.isSome (@empty α β var) = true := not_mem_empty
+
+lemma mem_update_of_ne (h : k ≠ k') (h₁ : k ∈ m[k'] := v) : k ∈ m := by
+  rw [mem_def] at *; unfold update at h₁; aesop
+
+lemma mem_fromList {l : List (α × β)} : k ∈ fromList l ↔ k ∈ l.map Prod.fst := by
+  induction l with
+    | nil => simp
+    | cons hd tl ih =>
+        rcases hd with ⟨k', v'⟩
+        rw [List.map_cons, List.mem_cons, ←ih]; simp
+        apply Iff.intro <;> intros h <;> {
+          rw [mem_def] at h ⊢; unfold Map.update at *
+          aesop
+        }
+
+lemma mem_unroll_assignment : k ∈ m[k'] := v ↔ (k = k' ∨ k ∈ m) := by
+  simp [update, mem_def]; aesop
+
+end Map
+
+end Map
+
+instance {α β : Type} [DecidableEq α] {m : Map α β} {k : α} : Decidable (k ∈ m) :=
+  Map.mem_def ▸ inferInstance
+
+section tactics
+
+open Lean Elab Tactic
+
+-- Probably the simplest way to decide membership for maps that contain metavariables.
+-- E.g. 42 ∈ empty[42] := k.succ.
+elab "decide_mem_map" : tactic => do
+  evalTactic <| ← `(
+    tactic| repeat ( first | apply Map.mem_update_self | apply Map.mem_skip )
+  )
+
+end tactics
+
+end Risc0
