lakefile.lean
@@ -1,18 +1,18 @@
 import Lake
 open Lake DSL
 
-package is0 {
+package risc0 {
   -- add package configuration options here
 }
 
-lean_lib Is0 {
+lean_lib Risc0 {
   -- add library configuration options here
 }
 
 require mathlib from git
-  "https://github.com/leanprover-community/mathlib4.git"
+  "https://github.com/leanprover-community/mathlib4.git" @ "c59c263ccfa439765d0e990b91ab9f4e09541375"
 
 @[default_target]
-lean_exe is0 {
+lean_exe risc0 {
   root := `Main
 }
